pcuic/theories/PCUICContextConversion.v
@@ -1,6 +1,6 @@
 (* Distributed under the terms of the MIT license. *)
 From MetaCoq.Template Require Import config utils.
-From MetaCoq.PCUIC Require Import PCUICAst PCUICAstUtils
+From MetaCoq.PCUIC Require Import PCUICAst PCUICOnOne PCUICAstUtils
      PCUICLiftSubst PCUICTyping PCUICWeakening PCUICCases
      PCUICCumulativity PCUICReduction
      PCUICParallelReduction PCUICEquality PCUICUnivSubstitutionConv
