pcuic/theories/PCUICParallelReduction.v
@@ -1,7 +1,7 @@
 (* Distributed under the terms of the MIT license. *)
 Require Import RelationClasses CRelationClasses.
 From MetaCoq.Template Require Import config utils.
-From MetaCoq.PCUIC Require Import PCUICUtils PCUICAst PCUICAstUtils PCUICDepth PCUICCases
+From MetaCoq.PCUIC Require Import PCUICUtils PCUICOnOne PCUICAst PCUICAstUtils PCUICDepth PCUICCases
      PCUICLiftSubst PCUICUnivSubst PCUICReduction PCUICTyping
      PCUICSigmaCalculus PCUICWeakeningEnvConv PCUICInduction
      PCUICRenameDef PCUICRenameConv PCUICInstDef PCUICInstConv PCUICOnFreeVars PCUICWeakening
